src/cbor/raw/pulse/everparse/CBOR.Pulse.Raw.Match.Serialized.fst
@@ -8,13 +8,13 @@ module U64 = FStar.UInt64
 let cbor_match_serialized_payload_array
   c p r
 = exists* n (r': nlist n raw_data_item) .
-    pts_to_serialized (tot_serialize_nlist n serialize_raw_data_item) c #p r' **
+    pts_to_serialized (serialize_nlist n serialize_raw_data_item) c #p r' **
     pure (r == r')
 
 let cbor_match_serialized_payload_map
   c p r
 = exists* n (r' : nlist n (raw_data_item & raw_data_item)) .
-    pts_to_serialized (tot_serialize_nlist n (serialize_raw_data_item `tot_serialize_nondep_then` serialize_raw_data_item)) c #p r' **
+    pts_to_serialized (serialize_nlist n (serialize_raw_data_item `serialize_nondep_then` serialize_raw_data_item)) c #p r' **
     pure (r == r')
 
 let cbor_match_serialized_payload_tagged
